Added oracle parameter to nat.partrec definition

src/computability/partrec.lean
@@ -144,7 +144,7 @@ theorem rfind_opt_mono {α} {f : ℕ → option α}
   simp at this, simp [this, get_mem]
 end⟩
 
-inductive partrec : (ℕ →. ℕ) → Prop
+inductive partrec (O : ℕ → ℕ) : (ℕ →. ℕ) → Prop
 | zero : partrec (pure 0)
 | succ : partrec succ
 | left : partrec ↑(λ n : ℕ, n.unpair.1)
@@ -155,17 +155,18 @@ inductive partrec : (ℕ →. ℕ) → Prop
     n.elim (f a) (λ y IH, do i ← IH, g (mkpair a (mkpair y i)))))
 | rfind {f} : partrec f → partrec (λ a,
     rfind (λ n, (λ m, m = 0) <$> f (mkpair a n)))
+| oracle : partrec O
 
 namespace partrec
 
-theorem of_eq {f g : ℕ →. ℕ} (hf : partrec f) (H : ∀ n, f n = g n) : partrec g :=
+theorem of_eq {O : ℕ → ℕ} {f g : ℕ →. ℕ} (hf : partrec O f) (H : ∀ n, f n = g n) : partrec O g :=
 (funext H : f = g) ▸ hf
 
-theorem of_eq_tot {f : ℕ →. ℕ} {g : ℕ → ℕ}
-  (hf : partrec f) (H : ∀ n, g n ∈ f n) : partrec g :=
+theorem of_eq_tot {O : ℕ → ℕ} {f : ℕ →. ℕ} {g : ℕ → ℕ}
+  (hf : partrec O f) (H : ∀ n, g n ∈ f n) : partrec O g :=
 hf.of_eq (λ n, eq_some_iff.2 (H n))
 
-theorem of_primrec {f : ℕ → ℕ} (hf : primrec f) : partrec f :=
+theorem of_primrec {O : ℕ → ℕ} {f : ℕ → ℕ} (hf : primrec f) : partrec O f :=
 begin
   induction hf,
   case nat.primrec.zero { exact zero },
@@ -185,22 +186,22 @@ begin
     simp, exact ⟨_, IH, rfl⟩ },
 end
 
-protected theorem some : partrec some := of_primrec primrec.id
+protected theorem some {O : ℕ → ℕ} : partrec O some := of_primrec primrec.id
 
-theorem none : partrec (λ n, none) :=
+theorem none {O : ℕ → ℕ} : partrec O (λ n, none) :=
 (of_primrec (nat.primrec.const 1)).rfind.of_eq $
 λ n, eq_none_iff.2 $ λ a ⟨h, e⟩, by simpa using h
 
-theorem prec' {f g h}
-  (hf : partrec f) (hg : partrec g) (hh : partrec h) :
-  partrec (λ a, (f a).bind (λ n, n.elim (g a)
+theorem prec' {O : ℕ → ℕ} {f g h}
+  (hf : partrec O f) (hg : partrec O g) (hh : partrec O h) :
+  partrec O (λ a, (f a).bind (λ n, n.elim (g a)
     (λ y IH, do i ← IH, h (mkpair a (mkpair y i))))) :=
 ((prec hg hh).comp (pair partrec.some hf)).of_eq $
 λ a, ext $ λ s, by simp [(<*>)]; exact
 ⟨λ ⟨n, h₁, h₂⟩, ⟨_, ⟨_, h₁, rfl⟩, by simpa using h₂⟩,
  λ ⟨_, ⟨n, h₁, rfl⟩, h₂⟩, ⟨_, h₁, by simpa using h₂⟩⟩
 
-theorem ppred : partrec (λ n, ppred n) :=
+theorem ppred {O : ℕ → ℕ} : partrec O (λ n, ppred n) :=
 have primrec₂ (λ n m, if n = nat.succ m then 0 else 1),
 from (primrec.ite
   (@@primrec_rel.comp _ _ _ _ _ _ _ primrec.eq
@@ -220,104 +221,104 @@ end partrec
 
 end nat
 
-def partrec {α σ} [primcodable α] [primcodable σ]
-  (f : α →. σ) := nat.partrec (λ n,
+def partrec {α σ} [primcodable α] [primcodable σ] (O : ℕ → ℕ)
+  (f : α →. σ) := nat.partrec O (λ n,
   roption.bind (decode α n) (λ a, (f a).map encode))
 
 def partrec₂ {α β σ} [primcodable α] [primcodable β] [primcodable σ]
-  (f : α → β →. σ) := partrec (λ p : α × β, f p.1 p.2)
+  (O : ℕ → ℕ) (f : α → β →. σ) := partrec O (λ p : α × β, f p.1 p.2)
 
-def computable {α σ} [primcodable α] [primcodable σ] (f : α → σ) := partrec (f : α →. σ)
+def computable {α σ} [primcodable α] [primcodable σ] (O : ℕ → ℕ) (f : α → σ) := partrec O (f : α →. σ)
 
 def computable₂ {α β σ} [primcodable α] [primcodable β] [primcodable σ]
-  (f : α → β → σ) := computable (λ p : α × β, f p.1 p.2)
+  (O : ℕ → ℕ) (f : α → β → σ) := computable O (λ p : α × β, f p.1 p.2)
 
 theorem primrec.to_comp {α σ} [primcodable α] [primcodable σ]
-  {f : α → σ} (hf : primrec f) : computable f :=
+  {O : ℕ → ℕ} {f : α → σ} (hf : primrec f) : computable O f :=
 (nat.partrec.ppred.comp (nat.partrec.of_primrec hf)).of_eq $
 λ n, by simp; cases decode α n; simp
 
 theorem primrec₂.to_comp {α β σ} [primcodable α] [primcodable β] [primcodable σ]
-  {f : α → β → σ} (hf : primrec₂ f) : computable₂ f := hf.to_comp
+  {O : ℕ → ℕ} {f : α → β → σ} (hf : primrec₂ f) : computable₂ O f := hf.to_comp
 
 theorem computable.part {α σ} [primcodable α] [primcodable σ]
-  {f : α → σ} (hf : computable f) : partrec (f : α →. σ) := hf
+  {O : ℕ → ℕ} {f : α → σ} (hf : computable O f) : partrec O (f : α →. σ) := hf
 
 theorem computable₂.part {α β σ} [primcodable α] [primcodable β] [primcodable σ]
-  {f : α → β → σ} (hf : computable₂ f) : partrec₂ (λ a, (f a : β →. σ)) := hf
+  {O : ℕ → ℕ} {f : α → β → σ} (hf : computable₂ O f) : partrec₂ O (λ a, (f a : β →. σ)) := hf
 
 namespace computable
 variables {α : Type*} {β : Type*} {γ : Type*} {σ : Type*}
 variables [primcodable α] [primcodable β] [primcodable γ] [primcodable σ]
 
-theorem of_eq {f g : α → σ} (hf : computable f) (H : ∀ n, f n = g n) : computable g :=
+theorem of_eq {O : ℕ → ℕ} {f g : α → σ} (hf : computable O f) (H : ∀ n, f n = g n) : computable O g :=
 (funext H : f = g) ▸ hf
 
-theorem const (s : σ) : computable (λ a : α, s) :=
+theorem const (s : σ) {O : ℕ → ℕ} : computable O (λ a : α, s) :=
 (primrec.const _).to_comp
 
-theorem of_option {f : α → option β}
-  (hf : computable f) : partrec (λ a, (f a : roption β)) :=
+theorem of_option {O : ℕ → ℕ} {f : α → option β}
+  (hf : computable O f) : partrec O (λ a, (f a : roption β)) :=
 (nat.partrec.ppred.comp hf).of_eq $ λ n, begin
   cases decode α n with a; simp,
   cases f a with b; simp
 end
 
-theorem to₂ {f : α × β → σ} (hf : computable f) : computable₂ (λ a b, f (a, b)) :=
+theorem to₂ {O : ℕ → ℕ} {f : α × β → σ} (hf : computable O f) : computable₂ O (λ a b, f (a, b)) :=
 hf.of_eq $ λ ⟨a, b⟩, rfl
 
-protected theorem id : computable (@id α) := primrec.id.to_comp
+protected theorem id {O : ℕ → ℕ} : computable O (@id α) := primrec.id.to_comp
 
-theorem fst : computable (@prod.fst α β) := primrec.fst.to_comp
+theorem fst {O : ℕ → ℕ} : computable O (@prod.fst α β) := primrec.fst.to_comp
 
-theorem snd : computable (@prod.snd α β) := primrec.snd.to_comp
+theorem snd {O : ℕ → ℕ} : computable O (@prod.snd α β) := primrec.snd.to_comp
 
-theorem pair {f : α → β} {g : α → γ}
-  (hf : computable f) (hg : computable g) : computable (λ a, (f a, g a)) :=
+theorem pair {O : ℕ → ℕ} {f : α → β} {g : α → γ}
+  (hf : computable O f) (hg : computable O g) : computable O (λ a, (f a, g a)) :=
 (hf.pair hg).of_eq $
 λ n, by cases decode α n; simp [(<*>)]
 
-theorem unpair : computable nat.unpair := primrec.unpair.to_comp
+theorem unpair {O : ℕ → ℕ} : computable O nat.unpair := primrec.unpair.to_comp
 
-theorem succ : computable nat.succ := primrec.succ.to_comp
-theorem pred : computable nat.pred := primrec.pred.to_comp
-theorem nat_bodd : computable nat.bodd := primrec.nat_bodd.to_comp
-theorem nat_div2 : computable nat.div2 := primrec.nat_div2.to_comp
+theorem succ {O : ℕ → ℕ} : computable O nat.succ := primrec.succ.to_comp
+theorem pred {O : ℕ → ℕ} : computable O nat.pred := primrec.pred.to_comp
+theorem nat_bodd {O : ℕ → ℕ} : computable O nat.bodd := primrec.nat_bodd.to_comp
+theorem nat_div2 {O : ℕ → ℕ} : computable O nat.div2 := primrec.nat_div2.to_comp
 
-theorem sum_inl : computable (@sum.inl α β) := primrec.sum_inl.to_comp
-theorem sum_inr : computable (@sum.inr α β) := primrec.sum_inr.to_comp
+theorem sum_inl {O : ℕ → ℕ} : computable O (@sum.inl α β) := primrec.sum_inl.to_comp
+theorem sum_inr {O : ℕ → ℕ} : computable O (@sum.inr α β) := primrec.sum_inr.to_comp
 
-theorem list_cons : computable₂ (@list.cons α) := primrec.list_cons.to_comp
-theorem list_reverse : computable (@list.reverse α) := primrec.list_reverse.to_comp
-theorem list_nth : computable₂ (@list.nth α) := primrec.list_nth.to_comp
-theorem list_append : computable₂ ((++) : list α → list α → list α) := primrec.list_append.to_comp
-theorem list_concat : computable₂ (λ l (a:α), l ++ [a]) := primrec.list_concat.to_comp
-theorem list_length : computable (@list.length α) := primrec.list_length.to_comp
+theorem list_cons {O : ℕ → ℕ} : computable₂ O (@list.cons α) := primrec.list_cons.to_comp
+theorem list_reverse {O : ℕ → ℕ} : computable O (@list.reverse α) := primrec.list_reverse.to_comp
+theorem list_nth {O : ℕ → ℕ} : computable₂ O (@list.nth α) := primrec.list_nth.to_comp
+theorem list_append {O : ℕ → ℕ} : computable₂ O ((++) : list α → list α → list α) := primrec.list_append.to_comp
+theorem list_concat {O : ℕ → ℕ} : computable₂ O (λ l (a:α), l ++ [a]) := primrec.list_concat.to_comp
+theorem list_length {O : ℕ → ℕ} : computable O (@list.length α) := primrec.list_length.to_comp
 
-theorem vector_cons {n} : computable₂ (@vector.cons α n) := primrec.vector_cons.to_comp
-theorem vector_to_list {n} : computable (@vector.to_list α n) := primrec.vector_to_list.to_comp
-theorem vector_length {n} : computable (@vector.length α n) := primrec.vector_length.to_comp
-theorem vector_head {n} : computable (@vector.head α n) := primrec.vector_head.to_comp
-theorem vector_tail {n} : computable (@vector.tail α n) := primrec.vector_tail.to_comp
-theorem vector_nth {n} : computable₂ (@vector.nth α n) := primrec.vector_nth.to_comp
-theorem vector_nth' {n} : computable (@vector.nth α n) := primrec.vector_nth'.to_comp
-theorem vector_of_fn' {n} : computable (@vector.of_fn α n) := primrec.vector_of_fn'.to_comp
+theorem vector_cons {n} {O : ℕ → ℕ} : computable₂ O (@vector.cons α n) := primrec.vector_cons.to_comp
+theorem vector_to_list {n} {O : ℕ → ℕ} : computable O (@vector.to_list α n) := primrec.vector_to_list.to_comp
+theorem vector_length {n} {O : ℕ → ℕ} : computable O (@vector.length α n) := primrec.vector_length.to_comp
+theorem vector_head {n} {O : ℕ → ℕ} : computable O (@vector.head α n) := primrec.vector_head.to_comp
+theorem vector_tail {n} {O : ℕ → ℕ} : computable O (@vector.tail α n) := primrec.vector_tail.to_comp
+theorem vector_nth {n} {O : ℕ → ℕ} : computable₂ O (@vector.nth α n) := primrec.vector_nth.to_comp
+theorem vector_nth' {n} {O : ℕ → ℕ} : computable O (@vector.nth α n) := primrec.vector_nth'.to_comp
+theorem vector_of_fn' {n} {O : ℕ → ℕ} : computable O (@vector.of_fn α n) := primrec.vector_of_fn'.to_comp
 
-theorem fin_app {n} : computable₂ (@id (fin n → σ)) := primrec.fin_app.to_comp
+theorem fin_app {n} {O : ℕ → ℕ} : computable₂ O (@id (fin n → σ)) := primrec.fin_app.to_comp
 
-protected theorem encode : computable (@encode α _) :=
+protected theorem encode {O : ℕ → ℕ} : computable O (@encode α _) :=
 primrec.encode.to_comp
 
-protected theorem decode : computable (decode α) :=
+protected theorem decode {O : ℕ → ℕ} : computable O (decode α) :=
 primrec.decode.to_comp
 
-protected theorem of_nat (α) [denumerable α] : computable (of_nat α) :=
+protected theorem of_nat (α) [denumerable α] {O : ℕ → ℕ} : computable O (of_nat α) :=
 (primrec.of_nat _).to_comp
 
-theorem encode_iff {f : α → σ} : computable (λ a, encode (f a)) ↔ computable f :=
+theorem encode_iff {O : ℕ → ℕ} {f : α → σ} : computable O (λ a, encode (f a)) ↔ computable O f :=
 iff.rfl
 
-theorem option_some : computable (@option.some α) :=
+theorem option_some {O : ℕ → ℕ} : computable O (@option.some α) :=
 primrec.option_some.to_comp
 
 end computable
@@ -328,40 +329,40 @@ variables [primcodable α] [primcodable β] [primcodable γ] [primcodable σ]
 
 open computable
 
-theorem of_eq {f g : α →. σ} (hf : partrec f) (H : ∀ n, f n = g n) : partrec g :=
+theorem of_eq {O : ℕ → ℕ} {f g : α →. σ} (hf : partrec O f) (H : ∀ n, f n = g n) : partrec O g :=
 (funext H : f = g) ▸ hf
 
-theorem of_eq_tot {f : α →. σ} {g : α → σ}
-  (hf : partrec f) (H : ∀ n, g n ∈ f n) : computable g :=
+theorem of_eq_tot {O : ℕ → ℕ} {f : α →. σ} {g : α → σ}
+  (hf : partrec O f) (H : ∀ n, g n ∈ f n) : computable O g :=
 hf.of_eq (λ a, eq_some_iff.2 (H a))
 
-theorem none : partrec (λ a : α, @roption.none σ) :=
+theorem none {O : ℕ → ℕ} : partrec O (λ a : α, @roption.none σ) :=
 nat.partrec.none.of_eq $ λ n, by cases decode α n; simp
 
-protected theorem some : partrec (@roption.some α) := computable.id
+protected theorem some {O : ℕ → ℕ} : partrec O (@roption.some α) := computable.id
 
-theorem const' (s : roption σ) : partrec (λ a : α, s) :=
+theorem const' (s : roption σ) {O : ℕ → ℕ} : partrec O (λ a : α, s) :=
 by haveI := classical.dec s.dom; exact
 (of_option (const (to_option s))).of_eq (λ a, of_to_option s)
 
-protected theorem bind {f : α →. β} {g : α → β →. σ}
-  (hf : partrec f) (hg : partrec₂ g) : partrec (λ a, (f a).bind (g a)) :=
+protected theorem bind {O : ℕ → ℕ} {f : α →. β} {g : α → β →. σ}
+  (hf : partrec O f) (hg : partrec₂ O g) : partrec O (λ a, (f a).bind (g a)) :=
 (hg.comp (nat.partrec.some.pair hf)).of_eq $
 λ n, by simp [(<*>)]; cases e : decode α n with a;
   simp [e, encodek]
 
-theorem map {f : α →. β} {g : α → β → σ}
-  (hf : partrec f) (hg : computable₂ g) : partrec (λ a, (f a).map (g a)) :=
+theorem map (O : ℕ → ℕ) {f : α →. β} {g : α → β → σ}
+  (hf : partrec O f) (hg : computable₂ O g) : partrec O (λ a, (f a).map (g a)) :=
 by simpa [bind_some_eq_map] using
-   @@partrec.bind _ _ _ (λ a b, roption.some (g a b)) hf hg
+   @@partrec.bind _ _ _ _ (λ a b, roption.some (g a b)) hf hg
 
-theorem to₂ {f : α × β →. σ} (hf : partrec f) : partrec₂ (λ a b, f (a, b)) :=
+theorem to₂ {O : ℕ → ℕ} {f : α × β →. σ} (hf : partrec O f) : partrec₂ O (λ a b, f (a, b)) :=
 hf.of_eq $ λ ⟨a, b⟩, rfl
 
 theorem nat_elim
-  {f : α → ℕ} {g : α →. σ} {h : α → ℕ × σ →. σ}
-  (hf : computable f) (hg : partrec g) (hh : partrec₂ h) :
-  partrec (λ a, (f a).elim (g a) (λ y IH, IH.bind (λ i, h a (y, i)))) :=
+  {O : ℕ → ℕ} {f : α → ℕ} {g : α →. σ} {h : α → ℕ × σ →. σ}
+  (hf : computable O f) (hg : partrec O g) (hh : partrec₂ O h) :
+  partrec O (λ a, (f a).elim (g a) (λ y IH, IH.bind (λ i, h a (y, i)))) :=
 (nat.partrec.prec' hf hg hh).of_eq $ λ n, begin
   cases e : decode α n with a; simp [e],
   induction f a with m IH; simp,
@@ -370,16 +371,16 @@ theorem nat_elim
   simp [encodek]
 end
 
-theorem comp {f : β →. σ} {g : α → β}
-  (hf : partrec f) (hg : computable g) : partrec (λ a, f (g a)) :=
+theorem comp {O : ℕ → ℕ} {f : β →. σ} {g : α → β}
+  (hf : partrec O f) (hg : computable O g) : partrec O (λ a, f (g a)) :=
 (hf.comp hg).of_eq $
 λ n, by simp; cases e : decode α n with a;
   simp [e, encodek]
 
-theorem nat_iff {f : ℕ →. ℕ} : partrec f ↔ nat.partrec f :=
+theorem nat_iff {O : ℕ → ℕ} {f : ℕ →. ℕ} : partrec O f ↔ nat.partrec O f :=
 by simp [partrec, map_id']
 
-theorem map_encode_iff {f : α →. σ} : partrec (λ a, (f a).map encode) ↔ partrec f :=
+theorem map_encode_iff {O : ℕ → ℕ} {f : α →. σ} : partrec O (λ a, (f a).map encode) ↔ partrec O f :=
 iff.rfl
 
 end partrec
@@ -388,22 +389,22 @@ namespace partrec₂
 variables {α : Type*} {β : Type*} {γ : Type*} {δ : Type*} {σ : Type*}
 variables [primcodable α] [primcodable β] [primcodable γ] [primcodable δ] [primcodable σ]
 
-theorem unpaired {f : ℕ → ℕ →. α} : partrec (nat.unpaired f) ↔ partrec₂ f :=
+theorem unpaired {O : ℕ → ℕ} {f : ℕ → ℕ →. α} : partrec O (nat.unpaired f) ↔ partrec₂ O f :=
 ⟨λ h, by simpa using h.comp primrec₂.mkpair.to_comp,
  λ h, h.comp primrec.unpair.to_comp⟩
 
-theorem unpaired' {f : ℕ → ℕ →. ℕ} : nat.partrec (nat.unpaired f) ↔ partrec₂ f :=
+theorem unpaired' {O : ℕ → ℕ} {f : ℕ → ℕ →. ℕ} : nat.partrec O (nat.unpaired f) ↔ partrec₂ O f :=
 partrec.nat_iff.symm.trans unpaired
 
 theorem comp
-  {f : β → γ →. σ} {g : α → β} {h : α → γ}
-  (hf : partrec₂ f) (hg : computable g) (hh : computable h) :
-  partrec (λ a, f (g a) (h a)) := hf.comp (hg.pair hh)
+  {O : ℕ → ℕ} {f : β → γ →. σ} {g : α → β} {h : α → γ}
+  (hf : partrec₂ O f) (hg : computable O g) (hh : computable O h) :
+  partrec O (λ a, f (g a) (h a)) := hf.comp (hg.pair hh)
 
 theorem comp₂
-  {f : γ → δ →. σ} {g : α → β → γ} {h : α → β → δ}
-  (hf : partrec₂ f) (hg : computable₂ g) (hh : computable₂ h) :
-  partrec₂ (λ a b, f (g a b) (h a b)) := hf.comp hg hh
+  {O : ℕ → ℕ} {f : γ → δ →. σ} {g : α → β → γ} {h : α → β → δ}
+  (hf : partrec₂ O f) (hg : computable₂ O g) (hh : computable₂ O h) :
+  partrec₂ O (λ a b, f (g a b) (h a b)) := hf.comp hg hh
 
 end partrec₂
 
@@ -411,13 +412,13 @@ namespace computable
 variables {α : Type*} {β : Type*} {γ : Type*} {σ : Type*}
 variables [primcodable α] [primcodable β] [primcodable γ] [primcodable σ]
 
-theorem comp {f : β → σ} {g : α → β}
-  (hf : computable f) (hg : computable g) :
-  computable (λ a, f (g a)) := hf.comp hg
+theorem comp {O : ℕ → ℕ} {f : β → σ} {g : α → β}
+  (hf : computable O f) (hg : computable O g) :
+  computable O (λ a, f (g a)) := hf.comp hg
 
-theorem comp₂ {f : γ → σ} {g : α → β → γ}
-  (hf : computable f) (hg : computable₂ g) :
-  computable₂ (λ a b, f (g a b)) := hf.comp hg
+theorem comp₂ {O : ℕ → ℕ} {f : γ → σ} {g : α → β → γ}
+  (hf : computable O f) (hg : computable₂ O g) :
+  computable₂ O (λ a b, f (g a b)) := hf.comp hg
 
 end computable
 
@@ -426,14 +427,14 @@ variables {α : Type*} {β : Type*} {γ : Type*} {δ : Type*} {σ : Type*}
 variables [primcodable α] [primcodable β] [primcodable γ] [primcodable δ] [primcodable σ]
 
 theorem comp
-  {f : β → γ → σ} {g : α → β} {h : α → γ}
-  (hf : computable₂ f) (hg : computable g) (hh : computable h) :
-  computable (λ a, f (g a) (h a)) := hf.comp (hg.pair hh)
+  {O : ℕ → ℕ} {f : β → γ → σ} {g : α → β} {h : α → γ}
+  (hf : computable₂ O f) (hg : computable O g) (hh : computable O h) :
+  computable O (λ a, f (g a) (h a)) := hf.comp (hg.pair hh)
 
 theorem comp₂
-  {f : γ → δ → σ} {g : α → β → γ} {h : α → β → δ}
-  (hf : computable₂ f) (hg : computable₂ g) (hh : computable₂ h) :
-  computable₂ (λ a b, f (g a b) (h a b)) := hf.comp hg hh
+  {O : ℕ → ℕ} {f : γ → δ → σ} {g : α → β → γ} {h : α → β → δ}
+  (hf : computable₂ O f) (hg : computable₂ O g) (hh : computable₂ O h) :
+  computable₂ O (λ a b, f (g a b) (h a b)) := hf.comp hg hh
 
 end computable₂
 
@@ -443,9 +444,9 @@ variables [primcodable α] [primcodable β] [primcodable γ] [primcodable σ]
 
 open computable
 
-theorem rfind {p : α → ℕ →. bool} (hp : partrec₂ p) :
-  partrec (λ a, nat.rfind (p a)) :=
-(nat.partrec.rfind $ hp.map
+theorem rfind {O : ℕ → ℕ} {p : α → ℕ →. bool} (hp : partrec₂ O p) :
+  partrec O (λ a, nat.rfind (p a)) :=
+(nat.partrec.rfind $ hp.map O
   ((primrec.dom_bool (λ b, cond b 0 1))
     .comp primrec.snd).to₂.to_comp).of_eq $
 λ n, begin
@@ -457,15 +458,15 @@ theorem rfind {p : α → ℕ →. bool} (hp : partrec₂ p) :
   cases b; refl
 end
 
-theorem rfind_opt {f : α → ℕ → option σ} (hf : computable₂ f) :
-  partrec (λ a, nat.rfind_opt (f a)) :=
+theorem rfind_opt {O : ℕ → ℕ} {f : α → ℕ → option σ} (hf : computable₂ O f) :
+  partrec O (λ a, nat.rfind_opt (f a)) :=
 (rfind (primrec.option_is_some.to_comp.comp hf).part.to₂).bind
   (of_option hf)
 
 theorem nat_cases_right
-  {f : α → ℕ} {g : α → σ} {h : α → ℕ →. σ}
-  (hf : computable f) (hg : computable g) (hh : partrec₂ h) :
-  partrec (λ a, (f a).cases (some (g a)) (h a)) :=
+  {O : ℕ → ℕ} {f : α → ℕ} {g : α → σ} {h : α → ℕ →. σ}
+  (hf : computable O f) (hg : computable O g) (hh : partrec₂ O h) :
+  partrec O (λ a, (f a).cases (some (g a)) (h a)) :=
 (nat_elim hf hg (hh.comp fst (pred.comp $ hf.comp fst)).to₂).of_eq $
 λ a, begin
   simp, cases f a; simp,
@@ -477,15 +478,15 @@ theorem nat_cases_right
     exact ⟨⟨this n, H.fst⟩, H.snd⟩ }
 end
 
-theorem bind_decode2_iff {f : α →. σ} : partrec f ↔
-  nat.partrec (λ n, roption.bind (decode2 α n) (λ a, (f a).map encode)) :=
+theorem bind_decode2_iff {O : ℕ → ℕ} {f : α →. σ} : partrec O f ↔
+  nat.partrec O (λ n, roption.bind (decode2 α n) (λ a, (f a).map encode)) :=
 ⟨λ hf, nat_iff.1 $ (of_option primrec.decode2.to_comp).bind $
-  (map hf (computable.encode.comp snd).to₂).comp snd,
+  (map O hf (computable.encode.comp snd).to₂).comp snd,
 λ h, map_encode_iff.1 $ by simpa [encodek2]
-  using (nat_iff.2 h).comp (@computable.encode α _)⟩
+  using (nat_iff.2 h).comp (@computable.encode α _ _)⟩
 
-theorem vector_m_of_fn : ∀ {n} {f : fin n → α →. σ}, (∀ i, partrec (f i)) →
-  partrec (λ (a : α), vector.m_of_fn (λ i, f i a))
+theorem vector_m_of_fn {O : ℕ → ℕ} : ∀ {n} {f : fin n → α →. σ}, (∀ i, partrec O (f i)) →
+  partrec O (λ (a : α), vector.m_of_fn (λ i, f i a))
 | 0     f hf := const _
 | (n+1) f hf := by simp [vector.m_of_fn]; exact
   (hf 0).bind (partrec.bind ((vector_m_of_fn (λ i, hf i.succ)).comp fst)
@@ -501,12 +502,12 @@ namespace computable
 variables {α : Type*} {β : Type*} {γ : Type*} {σ : Type*}
 variables [primcodable α] [primcodable β] [primcodable γ] [primcodable σ]
 
-theorem option_some_iff {f : α → σ} : computable (λ a, some (f a)) ↔ computable f :=
+theorem option_some_iff {O : ℕ → ℕ} {f : α → σ} : computable O (λ a, some (f a)) ↔ computable O f :=
 ⟨λ h, encode_iff.1 $ primrec.pred.to_comp.comp $ encode_iff.2 h,
  option_some.comp⟩
 
-theorem bind_decode_iff {f : α → β → option σ} : computable₂ (λ a n,
-  (decode β n).bind (f a)) ↔ computable₂ f :=
+theorem bind_decode_iff {O : ℕ → ℕ} {f : α → β → option σ} : computable₂ O (λ a n,
+  (decode β n).bind (f a)) ↔ computable₂ O f :=
 ⟨λ hf, nat.partrec.of_eq
     (((partrec.nat_iff.2 (nat.partrec.ppred.comp $
         nat.partrec.of_primrec $ primcodable.prim β)).comp snd).bind
@@ -515,70 +516,70 @@ theorem bind_decode_iff {f : α → β → option σ} : computable₂ (λ a n,
     cases decode α n.unpair.1; simp;
     cases decode β n.unpair.2; simp,
 λ hf, begin
-  have : partrec (λ a : α × ℕ, (encode (decode β a.2)).cases
+  have : partrec O (λ a : α × ℕ, (encode (decode β a.2)).cases
     (some option.none) (λ n, roption.map (f a.1) (decode β n))) :=
   partrec.nat_cases_right (primrec.encdec.to_comp.comp snd)
-    (const none) ((of_option (computable.decode.comp snd)).map
+    (const none) ((of_option (computable.decode.comp snd)).map O
       (hf.comp (fst.comp $ fst.comp fst) snd).to₂),
   refine this.of_eq (λ a, _),
   simp, cases decode β a.2; simp [encodek]
 end⟩
 
-theorem map_decode_iff {f : α → β → σ} : computable₂ (λ a n,
-  (decode β n).map (f a)) ↔ computable₂ f :=
+theorem map_decode_iff {O : ℕ → ℕ} {f : α → β → σ} : computable₂ O (λ a n,
+  (decode β n).map (f a)) ↔ computable₂ O f :=
 bind_decode_iff.trans option_some_iff
 
 theorem nat_elim
-  {f : α → ℕ} {g : α → σ} {h : α → ℕ × σ → σ}
-  (hf : computable f) (hg : computable g) (hh : computable₂ h) :
-  computable (λ a, (f a).elim (g a) (λ y IH, h a (y, IH))) :=
+  {O : ℕ → ℕ} {f : α → ℕ} {g : α → σ} {h : α → ℕ × σ → σ}
+  (hf : computable O f) (hg : computable O g) (hh : computable₂ O h) :
+  computable O (λ a, (f a).elim (g a) (λ y IH, h a (y, IH))) :=
 (partrec.nat_elim hf hg hh.part).of_eq $
 λ a, by simp; induction f a; simp *
 
-theorem nat_cases {f : α → ℕ} {g : α → σ} {h : α → ℕ → σ}
-  (hf : computable f) (hg : computable g) (hh : computable₂ h) :
-  computable (λ a, (f a).cases (g a) (h a)) :=
+theorem nat_cases {O : ℕ → ℕ} {f : α → ℕ} {g : α → σ} {h : α → ℕ → σ}
+  (hf : computable O f) (hg : computable O g) (hh : computable₂ O h) :
+  computable O (λ a, (f a).cases (g a) (h a)) :=
 nat_elim hf hg (hh.comp fst $ fst.comp snd).to₂
 
-theorem cond {c : α → bool} {f : α → σ} {g : α → σ}
-  (hc : computable c) (hf : computable f) (hg : computable g) :
-  computable (λ a, cond (c a) (f a) (g a)) :=
+theorem cond {O : ℕ → ℕ} {c : α → bool} {f : α → σ} {g : α → σ}
+  (hc : computable O c) (hf : computable O f) (hg : computable O g) :
+  computable O (λ a, cond (c a) (f a) (g a)) :=
 (nat_cases (encode_iff.2 hc) hg (hf.comp fst).to₂).of_eq $
 λ a, by cases c a; refl
 
-theorem option_cases {o : α → option β} {f : α → σ} {g : α → β → σ}
-  (ho : computable o) (hf : computable f) (hg : computable₂ g) :
-  @computable _ σ _ _ (λ a, option.cases_on (o a) (f a) (g a)) :=
+theorem option_cases {O : ℕ → ℕ} {o : α → option β} {f : α → σ} {g : α → β → σ}
+  (ho : computable O o) (hf : computable O f) (hg : computable₂ O g) :
+  @computable  _ σ _ _ O (λ a, option.cases_on (o a) (f a) (g a)) :=
 option_some_iff.1 $
 (nat_cases (encode_iff.2 ho) (option_some_iff.2 hf)
     (map_decode_iff.2 hg)).of_eq $
 λ a, by cases o a; simp [encodek]; refl
 
-theorem option_bind {f : α → option β} {g : α → β → option σ}
-  (hf : computable f) (hg : computable₂ g) :
-  computable (λ a, (f a).bind (g a)) :=
+theorem option_bind {O : ℕ → ℕ} {f : α → option β} {g : α → β → option σ}
+  (hf : computable O f) (hg : computable₂ O g) :
+  computable O (λ a, (f a).bind (g a)) :=
 (option_cases hf (const option.none) hg).of_eq $
 λ a, by cases f a; refl
 
-theorem option_map {f : α → option β} {g : α → β → σ}
-  (hf : computable f) (hg : computable₂ g) : computable (λ a, (f a).map (g a)) :=
+theorem option_map {O : ℕ → ℕ} {f : α → option β} {g : α → β → σ}
+  (hf : computable O f) (hg : computable₂ O g) : computable O (λ a, (f a).map (g a)) :=
 option_bind hf (option_some.comp₂ hg)
 
-theorem option_get_or_else {f : α → option β} {g : α → β}
-  (hf : computable f) (hg : computable g) :
-  computable (λ a, (f a).get_or_else (g a)) :=
-(computable.option_cases hf hg (show computable₂ (λ a b, b), from computable.snd)).of_eq $
+theorem option_get_or_else {O : ℕ → ℕ} {f : α → option β} {g : α → β}
+  (hf : computable O f) (hg : computable O g) :
+  computable O (λ a, (f a).get_or_else (g a)) :=
+(computable.option_cases hf hg (show computable₂ O (λ a b, b), from computable.snd)).of_eq $
 λ a, by cases f a; refl
 
-theorem subtype_mk {f : α → β} {p : β → Prop} [decidable_pred p] {h : ∀ a, p (f a)}
-    (hp : primrec_pred p) (hf : computable f) :
-  @computable _ _ _ (primcodable.subtype hp) (λ a, (⟨f a, h a⟩ : subtype p)) :=
+theorem subtype_mk {O : ℕ → ℕ} {f : α → β} {p : β → Prop} [decidable_pred p] {h : ∀ a, p (f a)}
+    (hp : primrec_pred p) (hf : computable O f) :
+  @computable _ _ _  (primcodable.subtype hp) O (λ a, (⟨f a, h a⟩ : subtype p)) :=
 nat.partrec.of_eq hf $ λ n, by cases decode α n; simp [subtype.encode_eq]
 
 theorem sum_cases
-  {f : α → β ⊕ γ} {g : α → β → σ} {h : α → γ → σ}
-  (hf : computable f) (hg : computable₂ g) (hh : computable₂ h) :
-  @computable _ σ _ _ (λ a, sum.cases_on (f a) (g a) (h a)) :=
+  {O : ℕ → ℕ} {f : α → β ⊕ γ} {g : α → β → σ} {h : α → γ → σ}
+  (hf : computable O f) (hg : computable₂ O g) (hh : computable₂ O h) :
+  @computable _ σ _ _ O (λ a, sum.cases_on (f a) (g a) (h a)) :=
 option_some_iff.1 $
 (cond (nat_bodd.comp $ encode_iff.2 hf)
   (option_map (computable.decode.comp $ nat_div2.comp $ encode_iff.2 hf) hh)
@@ -587,9 +588,9 @@ option_some_iff.1 $
   simp [nat.div2_bit, nat.bodd_bit, encodek]; refl
 
 theorem nat_strong_rec
-  (f : α → ℕ → σ) {g : α → list σ → option σ} (hg : computable₂ g)
-  (H : ∀ a n, g a ((list.range n).map (f a)) = some (f a n)) : computable₂ f :=
-suffices computable₂ (λ a n, (list.range n).map (f a)), from
+  {O : ℕ → ℕ} (f : α → ℕ → σ) {g : α → list σ → option σ} (hg : computable₂ O g)
+  (H : ∀ a n, g a ((list.range n).map (f a)) = some (f a n)) : computable₂ O f :=
+suffices computable₂ O (λ a n, (list.range n).map (f a)), from
   option_some_iff.1 $
   (list_nth.comp (this.comp fst (succ.comp snd)) snd).to₂.of_eq $
   λ a, by simp [list.nth_range (nat.lt_succ_self a.2)]; refl,
@@ -604,14 +605,14 @@ option_some_iff.1 $
   simp [IH, H, list.range_succ]
 end
 
-theorem list_of_fn : ∀ {n} {f : fin n → α → σ},
-  (∀ i, computable (f i)) → computable (λ a, list.of_fn (λ i, f i a))
+theorem list_of_fn {O : ℕ → ℕ} : ∀ {n} {f : fin n → α → σ},
+  (∀ i, computable O (f i)) → computable O (λ a, list.of_fn (λ i, f i a))
 | 0     f hf := const []
 | (n+1) f hf := by simp [list.of_fn_succ]; exact
   list_cons.comp (hf 0) (list_of_fn (λ i, hf i.succ))
 
-theorem vector_of_fn {n} {f : fin n → α → σ}
-  (hf : ∀ i, computable (f i)) : computable (λ a, vector.of_fn (λ i, f i a)) :=
+theorem vector_of_fn {n} {O : ℕ → ℕ} {f : fin n → α → σ}
+  (hf : ∀ i, computable O (f i)) : computable O (λ a, vector.of_fn (λ i, f i a)) :=
 (partrec.vector_m_of_fn hf).of_eq $ λ a, by simp
 
 end computable
@@ -622,27 +623,27 @@ variables [primcodable α] [primcodable β] [primcodable γ] [primcodable σ]
 
 open computable
 
-theorem option_some_iff {f : α →. σ} :
-  partrec (λ a, (f a).map option.some) ↔ partrec f :=
+theorem option_some_iff {O : ℕ → ℕ} {f : α →. σ} :
+  partrec O (λ a, (f a).map option.some) ↔ partrec O f :=
 ⟨λ h, (nat.partrec.ppred.comp h).of_eq $
    λ n, by simp [roption.bind_assoc, bind_some_eq_map],
- λ hf, hf.map (option_some.comp snd).to₂⟩
+ λ hf, hf.map O (option_some.comp snd).to₂⟩
 
-theorem option_cases_right {o : α → option β} {f : α → σ} {g : α → β →. σ}
-  (ho : computable o) (hf : computable f) (hg : partrec₂ g) :
-  @partrec _ σ _ _ (λ a, option.cases_on (o a) (some (f a)) (g a)) :=
-have partrec (λ (a : α), nat.cases (roption.some (f a))
+theorem option_cases_right {O : ℕ → ℕ} {o : α → option β} {f : α → σ} {g : α → β →. σ}
+  (ho : computable O o) (hf : computable O f) (hg : partrec₂ O g) :
+  @partrec _ σ _ _ O (λ a, option.cases_on (o a) (some (f a)) (g a)) :=
+have partrec O (λ (a : α), nat.cases (roption.some (f a))
   (λ n, roption.bind (decode β n) (g a)) (encode (o a))) :=
 nat_cases_right (encode_iff.2 ho) hf.part $
-  ((@computable.decode β _).comp snd).of_option.bind
+  ((@computable.decode β _ _).comp snd).of_option.bind
     (hg.comp (fst.comp fst) snd).to₂,
 this.of_eq $ λ a, by cases o a with b; simp [encodek]
 
 theorem sum_cases_right
-  {f : α → β ⊕ γ} {g : α → β → σ} {h : α → γ →. σ}
-  (hf : computable f) (hg : computable₂ g) (hh : partrec₂ h) :
-  @partrec _ σ _ _ (λ a, sum.cases_on (f a) (λ b, some (g a b)) (h a)) :=
-have partrec (λ a, (option.cases_on
+  {O : ℕ → ℕ} {f : α → β ⊕ γ} {g : α → β → σ} {h : α → γ →. σ}
+  (hf : computable O f) (hg : computable₂ O g) (hh : partrec₂ O h) :
+  @partrec _ σ _ _ O (λ a, sum.cases_on (f a) (λ b, some (g a b)) (h a)) :=
+have partrec O (λ a, (option.cases_on
   (sum.cases_on (f a) (λ b, option.none) option.some : option γ)
   (some (sum.cases_on (f a) (λ b, some (g a b))
      (λ c, option.none)))
@@ -654,15 +655,15 @@ option_cases_right
 option_some_iff.1 $ this.of_eq $ λ a, by cases f a; simp
 
 theorem sum_cases_left
-  {f : α → β ⊕ γ} {g : α → β →. σ} {h : α → γ → σ}
-  (hf : computable f) (hg : partrec₂ g) (hh : computable₂ h) :
-  @partrec _ σ _ _ (λ a, sum.cases_on (f a) (g a) (λ c, some (h a c))) :=
+  {O : ℕ → ℕ} {f : α → β ⊕ γ} {g : α → β →. σ} {h : α → γ → σ}
+  (hf : computable O f) (hg : partrec₂ O g) (hh : computable₂ O h) :
+  @partrec _ σ _ _ O (λ a, sum.cases_on (f a) (g a) (λ c, some (h a c))) :=
 (sum_cases_right (sum_cases hf
   (sum_inr.comp snd).to₂ (sum_inl.comp snd).to₂) hh hg).of_eq $
 λ a, by cases f a; simp
 
 private lemma fix_aux
-  {f : α →. σ ⊕ α} (hf : partrec f)
+  {O : ℕ → ℕ} {f : α →. σ ⊕ α} (hf : partrec O f)
   (a : α) (b : σ) :
   let F : α → ℕ →. σ ⊕ α := λ a n,
     n.elim (some (sum.inr a)) $ λ y IH, IH.bind $ λ s,
@@ -705,18 +706,18 @@ begin
 end
 
 theorem fix
-  {f : α →. σ ⊕ α} (hf : partrec f) : partrec (pfun.fix f) :=
+  {O : ℕ → ℕ} {f : α →. σ ⊕ α} (hf : partrec O f) : partrec O (pfun.fix f) :=
 let F : α → ℕ →. σ ⊕ α := λ a n,
   n.elim (some (sum.inr a)) $ λ y IH, IH.bind $ λ s,
   sum.cases_on s (λ _, roption.some s) f in
-have hF : partrec₂ F :=
+have hF : partrec₂ O F :=
 partrec.nat_elim snd (sum_inr.comp fst).part
   (sum_cases_right (snd.comp snd)
     (snd.comp $ snd.comp fst).to₂
     (hf.comp snd).to₂).to₂,
 let p := λ a n, @roption.map _ bool
   (λ s, sum.cases_on s (λ_, tt) (λ _, ff)) (F a n) in
-have hp : partrec₂ p := hF.map ((sum_cases computable.id
+have hp : partrec₂ O p := hF.map O ((sum_cases computable.id
   (const tt).to₂ (const ff).to₂).comp snd).to₂,
 (hp.rfind.bind (hF.bind
   (sum_cases_right snd snd.to₂ none.to₂).to₂).to₂).of_eq $
